coq/ZF/Meta/Sig.v
@@ -1,8 +1,0 @@
-Require Import Coq.Lists.List.
-Require Import Coq.Strings.String.
-
-Require Import ZF.Meta.Ty.
-
-Definition Sig : Type := string -> option (list Ty * Ty).
-
-Definition empty : Sig := fun _ => None.
