coq/ZF/Meta/HasTyDecl.v
@@ -1,0 +1,10 @@
+Require Import ZF.Meta.Decl.
+Require Import ZF.Meta.Env.
+Require Import ZF.Meta.HasTy.
+
+(* A declaration is well typed when its modeled body has its declared sort.     *)
+Definition HasTyDecl (e:Env) (d:Decl) : Prop :=
+  match Decl.body d with
+  | Some t => HasTy (Env.toSigs e) (Decl.ctx d) t (Decl.res d)
+  | None   => True
+  end.
