coq/ZF/Meta/Signature.v
@@ -1,0 +1,5 @@
+Require Import Coq.Lists.List.
+
+Require Import ZF.Meta.Ty.
+
+Definition Signature : Type := list Ty * Ty.
