coq/ZF/Meta/Sigs.v
@@ -1,0 +1,9 @@
+Require Import Coq.Lists.List.
+Require Import Coq.Strings.String.
+
+Require Import ZF.Meta.Ty.
+Require Import ZF.Meta.Signature.
+
+Definition Sigs : Type := string -> option Signature.
+
+Definition empty : Sigs := fun _ => None.
